Rebalancing of avl trees completed
	modified:   src/Avl_tree.v
	modified:   src/Binary_tree.v
	modified:   src/Core.v
	modified:   src/List_.v

src/Avl_tree.v
@@ -6,7 +6,6 @@ Import Equal.Notations.
 
 Set Implicit Arguments.
 
-
 Module Make (S0:SORTABLE).
 
 (*====================================*)
@@ -67,78 +66,111 @@ Module Make (S0:SORTABLE).
 (*====================================*)
 (** * Basic Definitions *)
 (*====================================*)
+  Section basic_definitions.
+
+    Definition Left_leaning  (t:T): Prop := Extra t B.left.
+    Definition Right_leaning (t:T): Prop := Extra t B.right.
+    Definition Balanced (t:T): Prop := Extra t B.balanced.
+    Definition Leaning (t:T): Prop := Left_leaning t \/ Right_leaning t.
 
 
-  Definition Left_leaning  (t:T): Prop := Extra t B.left.
-  Definition Right_leaning (t:T): Prop := Extra t B.right.
-  Definition Balanced (t:T): Prop := Extra t B.balanced.
-  Definition Leaning (t:T): Prop := Left_leaning t \/ Right_leaning t.
+    Theorem left_leaning_is_node:
+      forall (t:T), Left_leaning t -> Node t.
+    Proof
+      fun t ll => extra_is_node ll.
 
+    Theorem balanced_is_node:
+      forall (t:T), Balanced t -> Node t.
+    Proof
+      fun t bal => extra_is_node bal.
 
-  Theorem left_leaning_is_node:
-    forall (t:T), Left_leaning t -> Node t.
-  Proof
-    fun t ll => extra_is_node ll.
+    Theorem right_leaning_is_node:
+      forall (t:T), Right_leaning t -> Node t.
+    Proof
+      fun t bal => extra_is_node bal.
 
-  Theorem balanced_is_node:
-    forall (t:T), Balanced t -> Node t.
-  Proof
-    fun t bal => extra_is_node bal.
+    Theorem leaning_is_node:
+      forall t:T, Leaning t -> Node t.
+    Proof
+      fun t leaning =>
+        match leaning with
+        | or_introl p => left_leaning_is_node p
+        | or_intror p => right_leaning_is_node p
+        end.
 
-  Theorem right_leaning_is_node:
-    forall (t:T), Right_leaning t -> Node t.
-  Proof
-    fun t bal => extra_is_node bal.
+    Inductive Avl_height: T -> nat -> Prop :=
+    | empty_avl: Avl_height empty 0
+    | balanced_avl:
+        forall h a t1 t2,
+          Avl_height t1 h ->
+          Avl_height t2 h ->
+          Avl_height (node a B.balanced t1 t2) (1+h)
+    | left_avl:
+        forall h a t1 t2,
+          Avl_height t1 (1+h) ->
+          Avl_height t2 h ->
+          Avl_height (node a B.left t1 t2) (2+h)
+    | right_avl:
+        forall h a t1 t2,
+          Avl_height t1 h ->
+          Avl_height t2 (1+h) ->
+          Avl_height (node a B.right t1 t2) (2+h).
 
-  Theorem leaning_is_node:
-    forall t:T, Leaning t -> Node t.
-  Proof
-    fun t leaning =>
-      match leaning with
-      | or_introl p => left_leaning_is_node p
-      | or_intror p => right_leaning_is_node p
+    Theorem avl_height_is_height:
+      forall (t:T) (h:nat),
+        Avl_height t h ->
+        Height t h.
+    Proof
+      let maxhh  (h:nat): max h h = h := max_l h h (le_n h) in
+      let maxhh1 (h:nat): max h (1+h) = 1+h := max_r _ _ (le_S _ _ (le_n _)) in
+      let maxh1h (h:nat): max (1+h) h = 1+h := max_l _ _ (le_S _ _ (le_n _)) in
+      fix f t h avl :=
+      match avl in Avl_height t h
+            return Height t h
+      with
+      | empty_avl => empty_height
+      | balanced_avl a ph1 ph2 =>
+        Equal.rewrite
+          (maxhh _)
+          (fun x => Height  _ (1 + x))
+          (node_height a B.balanced (f _ _ ph1) (f _ _ ph2))
+      | left_avl a ph1 ph2 =>
+        Equal.rewrite
+          (maxh1h _)
+          (fun x => Height _ (1 + x))
+          (node_height a B.left (f _ _ ph1) (f _ _ ph2))
+      | right_avl a ph1 ph2 =>
+        Equal.rewrite
+          (maxhh1 _)
+          (fun x => Height _ (1 + x))
+          (node_height a B.right (f _ _ ph1) (f _ _ ph2))
       end.
 
-  Inductive Avl_height: T -> nat -> Prop :=
-  | empty_avl: Avl_height empty 0
-  | balanced_avl:
-      forall h a t1 t2,
-        Avl_height t1 h ->
-        Avl_height t2 h ->
-        Avl_height (node a B.balanced t1 t2) (1+h)
-  | left_avl:
-      forall h a t1 t2,
-        Avl_height t1 (1+h) ->
-        Avl_height t2 h ->
-        Avl_height (node a B.left t1 t2) (2+h)
-  | right_avl:
-      forall h a t1 t2,
-        Avl_height t1 h ->
-        Avl_height t2 (1+h) ->
-        Avl_height (node a B.right t1 t2) (2+h).
 
-  Definition Avl_tree (t:T): Prop :=
-    exists h, Avl_height t h.
 
-  Theorem avl_height_positive_is_node:
-    forall (t:T) (h:nat),
-      Avl_height t (S h) ->
-      Node t.
-  Proof
-    let f t h_ (avl:Avl_height t h_): forall h, S h = h_  -> Node t :=
-      (match avl in Avl_height t h_
-            return forall h, S h = h_ -> Node t with
-      | empty_avl =>
-        fun h eq => match Nat.successor_not_zero eq with end
-      | @balanced_avl h a t1 t2 ph1 ph2 =>
-        fun _ _ => I
-      | @left_avl h a t1 t2 ph1 ph2 =>
-        fun _ _ => I
-      | @right_avl h a t1 t2 ph1 ph2 =>
-        fun _ _ => I
-      end)
-    in
-    fun t h avl => f t (S h) avl h eq_refl .
+    Definition Avl_tree (t:T): Prop :=
+      Avl_height t (height t).
+
+    Theorem avl_height_positive_is_node:
+      forall (t:T) (h:nat),
+        Avl_height t (S h) ->
+        Node t.
+    Proof
+      let f t h_ (avl:Avl_height t h_): forall h, S h = h_  -> Node t :=
+          (match avl in Avl_height t h_
+                 return forall h, S h = h_ -> Node t with
+           | empty_avl =>
+             fun h eq => match Nat.successor_not_zero eq with end
+           | @balanced_avl h a t1 t2 ph1 ph2 =>
+             fun _ _ => I
+           | @left_avl h a t1 t2 ph1 ph2 =>
+             fun _ _ => I
+           | @right_avl h a t1 t2 ph1 ph2 =>
+             fun _ _ => I
+           end)
+      in
+      fun t h avl => f t (S h) avl h eq_refl .
+  End basic_definitions.
 
 
 
@@ -146,123 +178,251 @@ Module Make (S0:SORTABLE).
   (*====================================*)
   (** * Rebalancing *)
   (*====================================*)
-
-  Inductive Nearly_avl_left: A -> T -> T -> Prop :=
-  | lrl_nearly_avl_left:
-      (* lrl:
+  Section rebalancing.
+    Inductive Nearly_avl_left: A -> T -> T -> Prop :=
+    | lrl_nearly_avl_left:
+        (* lrl:
                       c
               a            t2
           t11     b        x
           x   t121 t122
               x
-       *)
-      forall h t11 t121 t122 t2 a b c,
-        Avl_height t11 (1+h) ->
-        Avl_height t121 (1+h) ->
-        Avl_height t122 h ->
-        Avl_height t2 (1+h) ->
-        Nearly_avl_left
-          c
-          (node a B.right t11 (node b B.left t121 t122))
-          t2
-  | lrr_nearly_avl_left:
-      (* lrl:
+         *)
+        forall h t11 t121 t122 t2 a b c,
+          Avl_height t11 (1+h) ->
+          Avl_height t121 (1+h) ->
+          Avl_height t122 h ->
+          Avl_height t2 (1+h) ->
+          Nearly_avl_left
+            c
+            (node a B.right t11 (node b B.left t121 t122))
+            t2
+    | lrr_nearly_avl_left:
+        (* lrl:
                       c
               a            t2
           t11     b        x
           x   t121 t122
                    x
-       *)
-      forall h t11 t121 t122 t2 a b c,
-        Avl_height t11 (1+h) ->
-        Avl_height t121 h ->
-        Avl_height t122 (1+h) ->
-        Avl_height t2 (1+h) ->
-        Nearly_avl_left
-          c
-          (node a B.right t11 (node b B.right t121 t122))
-          t2
-  | ll_nearly_avl_left:
-      (* ll:
+         *)
+        forall h t11 t121 t122 t2 a b c,
+          Avl_height t11 (1+h) ->
+          Avl_height t121 h ->
+          Avl_height t122 (1+h) ->
+          Avl_height t2 (1+h) ->
+          Nearly_avl_left
+            c
+            (node a B.right t11 (node b B.right t121 t122))
+            t2
+    | ll_nearly_avl_left:
+        (* ll:
                     c
               a          t2
           t11    t12
           x
-       *)
-      forall h t11 t12 t2 a c,
-        Avl_height t11 (1+h) ->
-        Avl_height t12 h ->
-        Avl_height t2  h ->
-        Nearly_avl_left
-          c
-          (node a B.left t11 t12)
-          t2.
+         *)
+        forall h t11 t12 t2 a c,
+          Avl_height t11 (1+h) ->
+          Avl_height t12 h ->
+          Avl_height t2  h ->
+          Nearly_avl_left
+            c
+            (node a B.left t11 t12)
+            t2.
 
 
 
 
-  Definition rebalance_left (c:A) (t1 t2:T): T :=
-    match t1  with
-    | empty =>
-      node c B.right empty t2
-    | node a B.right t11 (node b B.left t121 t122) =>
-      (* lrl:
+    Definition rebalance_left (c:A) (t1 t2:T): T :=
+      match t1  with
+      | empty =>
+        node c B.right empty t2
+      | node a B.right t11 (node b B.left t121 t122) =>
+        (* lrl:
                       c                               b
               a            t2                   a            c
           t11     b        x                 t11  t121   t122  t2
           x   t121 t122                      x    x            x
               x
-       *)
-      node
-        b B.balanced
-        (node a B.balanced t11 t121)
-        (node c B.right t122 t2)
-    | node a B.right t11 (node b B.right t121 t122) =>
-      (* lrr:
+         *)
+        node
+          b B.balanced
+          (node a B.balanced t11 t121)
+          (node c B.right t122 t2)
+      | node a B.right t11 (node b B.right t121 t122) =>
+        (* lrr:
                       c                               b
               a            t2                   a            c
           t11     b        x                 t11  t121   t122  t2
           x   t121 t122                      x           x     x
                    x
-       *)
-      node
-        b B.balanced
-        (node a B.left t11 t121)
-        (node c B.balanced t122 t2)
-    | node a bal t11 t12 =>
-      (* ll:
+         *)
+        node
+          b B.balanced
+          (node a B.left t11 t121)
+          (node c B.balanced t122 t2)
+      | node a bal t11 t12 =>
+        (* ll:
                     c                            a
               a          t2              t11            c
           t11    t12                     x          t12   t2
           x
-       *)
-      node a B.balanced t11 (node c B.balanced t12 t2)
-    end.
-
-
-  Theorem rebalance_left_rebalances:
-    forall (a:A) (t1 t2:T) (nearly:Nearly_avl_left a t1 t2),
-      Avl_tree (rebalance_left a t1 t2).
-  Proof
-    fun a t1 t2 nearly =>
-      match nearly in Nearly_avl_left a t1 t2
-            return Avl_tree (rebalance_left a t1 t2)
-      with
-      | lrl_nearly_avl_left a b c ph11 ph121 ph122 ph2 =>
-        let pa := balanced_avl a ph11 ph121 in
-        let pc := right_avl c ph122 ph2 in
-        let pb := balanced_avl b pa pc in
-        ex_intro _ _ pb
-      | lrr_nearly_avl_left a b c ph11 ph121 ph122 ph2 =>
-        let pa := left_avl a ph11 ph121 in
-        let pc := balanced_avl c ph122 ph2 in
-        let pb := balanced_avl b pa pc in
-        ex_intro _ _ pb
-      | ll_nearly_avl_left a c ph11 ph12 ph2 =>
-        let pc := balanced_avl c ph12 ph2 in
-        let pa := balanced_avl a ph11 pc in
-        ex_intro _ _ pa
+         *)
+        node a B.balanced t11 (node c B.balanced t12 t2)
       end.
 
 
+    Theorem rebalance_left_rebalances:
+      forall (a:A) (t1 t2:T) (nearly:Nearly_avl_left a t1 t2),
+        Avl_height (rebalance_left a t1 t2) (2 + height t2).
+    Proof
+      let rewrite h t1 t2 (ph1:Avl_height t1 h) (ph2:Avl_height t2 (2+h)) :=
+          Equal.rewrite
+            (height_is_only_height (avl_height_is_height ph1))
+            (fun x => Avl_height t2 (2 + x))
+            ph2
+      in
+      fun a t1 t2 nearly =>
+        match nearly in Nearly_avl_left a t1 t2
+              return Avl_height (rebalance_left a t1 t2) (2 + height t2)
+        with
+        | lrl_nearly_avl_left a b c ph11 ph121 ph122 ph2 =>
+          let pa := balanced_avl a ph11 ph121 in
+          let pc := right_avl c ph122 ph2 in
+          let pb := balanced_avl b pa pc in
+          rewrite _ _ _ ph2 pb
+        | lrr_nearly_avl_left a b c ph11 ph121 ph122 ph2 =>
+          let pa := left_avl a ph11 ph121 in
+          let pc := balanced_avl c ph122 ph2 in
+          let pb := balanced_avl b pa pc in
+          rewrite _ _ _ ph2 pb
+        | ll_nearly_avl_left a c ph11 ph12 ph2 =>
+          let pc := balanced_avl c ph12 ph2 in
+          let pa := balanced_avl a ph11 pc in
+          rewrite _ _ _ ph2 pa
+        end.
+
+
+    Inductive Nearly_avl_right: A -> T -> T -> Prop :=
+    | rll_nearly_avl_right:
+        (* rll:
+                   a
+           t1               c
+           x           b        t22
+                   t211 t212    x
+                   x
+         *)
+        forall h t1 t211 t212 t22 a b c,
+          Avl_height t1 (1+h) ->
+          Avl_height t211 (1+h) ->
+          Avl_height t212 h ->
+          Avl_height t22 (1+h) ->
+          Nearly_avl_right
+            a
+            t1
+            (node c B.left (node b B.left t211 t212) t22)
+    | rlr_nearly_avl_right:
+        (* rlr:
+                   a
+           t1               c
+           x           b        t22
+                   t211 t212    x
+                         x
+         *)
+        forall h t1 t211 t212 t22 a b c,
+          Avl_height t1 (1+h) ->
+          Avl_height t211 h ->
+          Avl_height t212 (1+h) ->
+          Avl_height t22 (1+h) ->
+          Nearly_avl_right
+            a
+            t1
+            (node c B.left (node b B.right t211 t212) t22)
+    | rr_nearly_avl_right:
+        (* rr:
+                   a
+           t1               c
+                       t21      t22
+                                x
+         *)
+        forall h t1 t21 t22 a c,
+          Avl_height t1 h ->
+          Avl_height t21 h ->
+          Avl_height t22 (1+h) ->
+          Nearly_avl_right
+            a
+            t1
+            (node c B.right t21 t22).
+
+
+
+    Definition rebalance_right (a:A) (t1 t2:T): T :=
+      match t2  with
+      | empty =>
+        node a B.left t1 empty
+      | node c B.left (node b B.left t211 t212) t21 =>
+        (* rll:
+                   a                                  b
+           t1               c                   a            c
+           x           b        t21          t1  t211    t212 t21
+                   t211 t212    x            x   x            x
+                   x
+         *)
+        node
+          b B.balanced
+          (node a B.balanced t1 t211)
+          (node c B.right t212 t21)
+      | node c B.left (node b B.right t211 t212) t22 =>
+        (* rlr:
+                   a                                  b
+           t1               c                   a            c
+           x           b        t22          t1  t211    t212 t22
+                   t211 t212    x            x           x    x
+                        x
+         *)
+        node
+          b B.balanced
+          (node a B.left t1 t211)
+          (node c B.balanced t212 t22)
+      | node c bal t21 t22 =>
+        (* rr:
+                   a                                  c
+           t1               c                   a          t22
+                       t21      t22          t1  t21       x
+                                x
+         *)
+        node c B.balanced (node a B.balanced t1 t21) t22
+      end.
+
+
+    Theorem rebalance_right_rebalances:
+      forall (a:A) (t1 t2:T) (nearly:Nearly_avl_right a t1 t2),
+        Avl_height (rebalance_right a t1 t2) (2 + height t1).
+    Proof
+      let rewrite h t1 t2 (ph1:Avl_height t1 h) (ph2:Avl_height t2 (2+h)) :=
+          Equal.rewrite
+            (height_is_only_height (avl_height_is_height ph1))
+            (fun x => Avl_height t2 (2 + x))
+            ph2
+      in
+      fun a t1 t2 nearly =>
+        match nearly in Nearly_avl_right a t1 t2
+              return Avl_height (rebalance_right a t1 t2) (2 + height t1)
+        with
+        | rll_nearly_avl_right a b c ph1 ph211 ph212 ph21 =>
+          let pa := balanced_avl a ph1 ph211 in
+          let pc := right_avl c ph212 ph21 in
+          let pb := balanced_avl b pa pc in
+          rewrite _ _ _ ph1 pb
+        | rlr_nearly_avl_right a b c ph1 ph211 ph212 ph22 =>
+          let pa := left_avl a ph1 ph211 in
+          let pc := balanced_avl c ph212 ph22 in
+          let pb := balanced_avl b pa pc in
+          rewrite _ _ _ ph1 pb
+        | rr_nearly_avl_right a c ph1 ph21 ph22 =>
+          let pa := balanced_avl a ph1 ph21 in
+          let pc := balanced_avl c pa ph22 in
+          rewrite _ _ _ ph1 pc
+        end.
+  End rebalancing.
 End Make.
